Tables/Data/Array/Disjoint.lean
@@ -1,0 +1,38 @@
+module
+
+public import Batteries.Data.List.Basic
+public import Tables.Data.Array.Pairwise
+
+public section
+
+namespace Array
+
+@[expose]
+def Disjoint {α} (a b : Array α) : Prop :=
+  a.toList.Disjoint b.toList
+
+namespace Disjoint
+
+variable {α} {a b : Array α}
+
+theorem iff_getElem_ne : a.Disjoint b ↔ ∀ i j, (_ : i < a.size) → (_ : j < b.size) → a[i] ≠ b[j] := by
+  unfold Disjoint List.Disjoint
+  simp only [List.mem_iff_getElem, Array.getElem_toList]
+  grind
+
+theorem iff_getElem_ne' : a.Disjoint b ↔ ∀ (i : Fin a.size) (j : Fin b.size), a[i.val] ≠ b[j.val] := by
+  rw [iff_getElem_ne]
+  apply Iff.intro
+  . intro h i j
+    exact h i.val j.val i.isLt j.isLt
+  . intro h i j hi hj
+    exact h ⟨i, hi⟩ ⟨j, hj⟩
+
+instance [DecidableEq α] : Decidable (Disjoint a b) :=
+  decidable_of_iff' _ iff_getElem_ne'
+
+end Disjoint
+
+end Array
+
+end
