Tables/Table/Raw/JoinLemmas.lean
@@ -90,30 +90,23 @@ theorem wfColumnNames_distinct (self : Raw) (h : self.WfColumnSize) (hwf : self.
 
 theorem wfColumnNames_crossJoin (self other : Raw) (h₁ : self.WfColumnSize) (h₂ : other.WfColumnSize)
     (hwf₁ : self.WfColumnNames) (hwf₂ : other.WfColumnNames)
-    (hdisjoint :
-      ∀ (i : Fin self.ncols) (j : Fin other.ncols),
-        (self.getColumn i.val i.isLt).name ≠ (other.getColumn j.val j.isLt).name) :
+    (hdisjoint : self.header.Disjoint other.header) :
     (crossJoin self other h₁ h₂).WfColumnNames := by
   rw [wfColumnNames_iff_schema_wf, crossJoin_schema]
-  exact Schema.wf_concat ((wfColumnNames_iff_schema_wf self).mp hwf₁) ((wfColumnNames_iff_schema_wf other).mp hwf₂)
-    fun i j => by
-      have isLt₁ : i.val < self.ncols := by simpa [schema_size_eq] using i.isLt
-      have isLt₂ : j.val < other.ncols := by simpa [schema_size_eq] using j.isLt
-      simpa [schema_getName_eq_getColumn_name i.val isLt₁, schema_getName_eq_getColumn_name j.val isLt₂]
-        using hdisjoint ⟨i, isLt₁⟩ ⟨j, isLt₂⟩
+  exact Schema.wf_concat
+    ((wfColumnNames_iff_schema_wf self).mp hwf₁)
+    ((wfColumnNames_iff_schema_wf other).mp hwf₂)
+    (by simpa [header_eq_schema_header] using hdisjoint)
 
 theorem wfColumnNames_leftJoin (self other : Raw) (keys : Array String)
     (h₁ : self.WfColumnSize) (h₂ : other.WfColumnSize)
     (hwf₁ : self.WfColumnNames) (hwf₂ : other.WfColumnNames)
-    (hdisjoint :
-      ∀ (i : Fin self.schema.size) (j : Fin (other.schema.selectNotByNames keys).size),
-        self.schema.getName i.val i.isLt ≠
-          (other.schema.selectNotByNames keys).getName j.val j.isLt) :
+    (hdisjoint : self.header.Disjoint (other.schema.selectNotByNames keys).header) :
     (leftJoin self other keys h₁ h₂).WfColumnNames := by
   rw [wfColumnNames_iff_schema_wf, leftJoin_schema]
   have hwfR : (other.schema.selectNotByNames keys).Wf := by
     simpa [Schema.selectNotByNames] using Schema.wf_filterByName ((wfColumnNames_iff_schema_wf other).mp hwf₂)
-  exact Schema.wf_concat ((wfColumnNames_iff_schema_wf self).mp hwf₁) hwfR hdisjoint
+  exact Schema.wf_concat ((wfColumnNames_iff_schema_wf self).mp hwf₁) hwfR (by simpa [header_eq_schema_header] using hdisjoint)
 
 theorem wfColumnNames_join {α} [BEq α] [Hashable α] (self other : Raw) (schema : Schema)
     (getKey₁ : Row → α) (getKey₂ : Row → α)
